generaling Interop.X64 to be parameterized by a relation on the final state passed in from the Vale.Decls layer

vale/code/arch/x64/interop/Vale.AsLowStar.Wrapper.fst
@@ -77,20 +77,42 @@ let core_create_lemma
                 LSig.vale_pre_hyp args va_s))
   = admit() //needs the definition of SL.state_to_S; not sure why its hidden in StateLemma
 
-let frame_mem_correspondence
+let frame_mem_correspondence_back
        (args:list arg)
        (h0:mem_roots args)
        (h1:mem_roots args)
        (va_s:V.va_state)
+       (l:B.loc)
  : Lemma
      (requires
        LSig.mem_correspondence args h1 va_s /\
-       B.modifies B.loc_none h0 h1)
+       B.modifies l h0 h1 /\
+       B.loc_disjoint (LSig.mk_modifies_loc args) l)
      (ensures
        LSig.mem_correspondence args h0 va_s)
  = admit()
 
 
+let frame_mem_correspondence
+       (args:list arg)
+       (h0:HS.mem)
+       (h1:HS.mem)
+       (va_s:V.va_state)
+       (l:B.loc)
+ : Lemma
+     (requires
+       LSig.mem_correspondence args h0 va_s /\
+       B.modifies l h0 h1 /\
+       B.loc_disjoint (LSig.mk_modifies_loc args) l)
+     (ensures
+       LSig.mem_correspondence args h1 va_s)
+ = admit()
+
+let args_fp (args:list arg)
+            (h0:mem_roots args)
+            (h1:HS.mem{HS.fresh_frame h0 h1})
+   : Lemma (B.loc_disjoint (LSig.mk_modifies_loc args) (B.loc_regions false (Set.singleton (HS.get_tip h1))))
+   = admit()
 
 module ST = FStar.HyperStack.ST
 assume
@@ -134,6 +156,76 @@ let fuel_irrelevance (c:TS.tainted_code)
 
 ////////////////////////////////////////////////////////////////////////////////
 
+let mem_correspondence_refl (args:list arg)
+                            (va_s:V.va_state)
+ : Lemma (ensures LSig.mem_correspondence args (Interop.Adapters.hs_of_mem va_s.VS.mem) va_s)
+ = admit()
+
+let state_to_S_mem
+      (va_s:_)
+      (s:_)
+      (mem:ME.mem)
+ : Lemma
+     (requires (
+       let open Interop.Adapters in
+       VL.state_eq_S (SL.state_to_S va_s) s /\
+       IM.down_mem
+         (hs_of_mem mem)
+         IA.addrs
+         (ptrs_of_mem mem) == s.TS.state.BS.mem))
+     (ensures
+       va_s.VS.mem == mem)
+ = admit()
+
+let vale_lemma_as_prediction
+          (code:V.va_code)
+          (args:IX64.arity_ok arg)
+          (num_stack_slots:nat)
+          (pre:VSig.vale_pre_tl [])
+          (post:VSig.vale_post_tl [])
+          (v:VSig.vale_sig_tl args (coerce code) pre post)
+          (h0:mem_roots args{LSig.(to_low_pre pre args (vale_pre_hyp args) (mem_correspondence args) num_stack_slots h0)})
+   : s0:TS.traceState ->
+     push_h0:mem_roots args ->
+     alloc_push_h0:mem_roots args ->
+     sb:IX64.stack_buffer{mem_roots_p alloc_push_h0 (IX64.arg_of_b8 sb::args)} ->
+     Ghost (nat & ME.mem)
+       (requires IX64.prediction_pre (coerce code) args h0 s0 push_h0 alloc_push_h0 sb)
+       (ensures (fun (fuel, final_mem) ->
+                Some? (TS.taint_eval_code (coerce code) fuel s0) /\ (
+                let sN = Some?.v (TS.taint_eval_code (coerce code) fuel s0) in
+                let va_s0 = create_initial_vale_state args alloc_push_h0 sb in
+                elim_nil pre va_s0 sb /\
+                (let va_s1, f = VSig.elim_vale_sig_nil v va_s0 sb in
+                 coerce f == fuel /\
+                 VL.state_eq_opt (Some (SL.state_to_S va_s1)) (Some sN)) /\
+                IX64.calling_conventions s0 sN)))
+   = fun s0 push_h0 alloc_push_h0 sb ->
+       let va_s0 = create_initial_vale_state args alloc_push_h0 sb in
+       core_create_lemma args alloc_push_h0 sb;
+       assert (SL.state_to_S va_s0 == s0);
+       B.fresh_frame_modifies h0 push_h0;
+       assert (B.modifies B.loc_none h0 alloc_push_h0);
+       assert (LSig.mem_correspondence args alloc_push_h0 va_s0);
+       frame_mem_correspondence_back args h0 alloc_push_h0 va_s0 B.loc_none;
+       assert (LSig.mem_correspondence args h0 va_s0);
+       assert (va_s0.VS.ok);
+       assert (LSig.vale_pre_hyp args va_s0);
+       assume (V.valid_stack_slots
+                va_s0.VS.mem
+                (VS.eval_reg MS.Rsp va_s0)
+                (as_vale_buffer sb)
+                num_stack_slots
+                va_s0.VS.memTaint);
+       assert (elim_nil pre va_s0 sb);
+       let va_s1, f = VSig.elim_vale_sig_nil v va_s0 sb in
+       assert (V.eval_code (coerce code) va_s0 f va_s1);
+       eval_code_rel (coerce code) va_s0 va_s1 f;
+       let Some s1 = TS.taint_eval_code (coerce code) (coerce f) s0 in
+       assert (VL.state_eq_opt (Some (SL.state_to_S va_s1)) (Some s1));
+       assert (IX64.calling_conventions s0 s1);
+       coerce f, va_s1.VS.mem
+
 let lowstar_lemma_base
           (code:V.va_code)
           (args:IX64.arity_ok arg)
@@ -154,13 +246,16 @@ let lowstar_lemma_base
     let As_lowstar_sig_ret push_h0 alloc_push_h0 stack_buf fuel final_mem = ret in
     let s0 = fst (create_initial_trusted_state args alloc_push_h0 stack_buf) in
     let Some s1 = TS.taint_eval_code (coerce code) fuel s0 in
+    assert (IM.down_mem (Interop.Adapters.hs_of_mem final_mem)
+                        (IA.addrs)
+                        (Interop.Adapters.ptrs_of_mem final_mem) == s1.TS.state.BS.mem);
     let va_s0 = create_initial_vale_state args alloc_push_h0 stack_buf in
     core_create_lemma args alloc_push_h0 stack_buf;
     assert (SL.state_to_S va_s0 == s0);
     B.fresh_frame_modifies h0 push_h0;
     assert (B.modifies B.loc_none h0 alloc_push_h0);
     assert (mem_correspondence args alloc_push_h0 va_s0);
-    frame_mem_correspondence args h0 alloc_push_h0 va_s0;
+    frame_mem_correspondence_back args h0 alloc_push_h0 va_s0 B.loc_none;
     assert (mem_correspondence args h0 va_s0);
     assert (va_s0.VS.ok);
     assert (vale_pre_hyp args va_s0);
@@ -180,36 +275,39 @@ let lowstar_lemma_base
     assert (VSig.vale_calling_conventions va_s0 va_s1);
     assert (elim_nil post va_s0 stack_buf va_s1 f);
     assert (ME.modifies (VSig.fp_of_args args) va_s0.VS.mem va_s1.VS.mem);
-    let h1_pre_pop // : mem_roots args
-      = Interop.Adapters.hs_of_mem final_mem in
-    assume (mem_correspondence args h1_pre_pop va_s1);
-//    let h1_pre = IM.down_mem
+    let h1_pre_pop = Interop.Adapters.hs_of_mem final_mem in
+    assert (IM.down_mem h1_pre_pop (IA.addrs) (Interop.Adapters.ptrs_of_mem final_mem) == s1.TS.state.BS.mem);
+    assume (va_s1.VS.mem == final_mem);
+    mem_correspondence_refl args va_s1;
     assert (HS.poppable h1_pre_pop);
     assert (h1 == HS.pop h1_pre_pop);
-    assume (mem_correspondence args h1 va_s1)
+    args_fp args h0 push_h0;
+    assert (HS.get_tip push_h0 == HS.get_tip h1_pre_pop);
+    B.popped_modifies h1_pre_pop h1;
+    frame_mem_correspondence args h1_pre_pop h1 va_s1 (B.loc_regions false (Set.singleton (HS.get_tip h1_pre_pop)))
 
-// let rec lowstar_lemma
-//           (dom:list td)
-//           (code:V.va_code)
-//           (args:list arg{List.length args + List.length dom < IX64.max_arity})
-//           (num_stack_slots:nat)
-//           (pre:VSig.vale_pre_tl dom)
-//           (post:VSig.vale_post_tl dom)
-//           (v:VSig.vale_sig_tl args (coerce code) pre post)
-//     : lowstar_lemma_typ code args num_stack_slots pre post
-//     = match dom with
-//       | [] ->
-//         lowstar_lemma_base code args num_stack_slots pre post v
-//       | hd::tl ->
-//         fun (x:td_as_type hd) ->
-//           lowstar_lemma
-//             tl
-//             code
-//             ((| hd, x |) :: args)
-//             num_stack_slots
-//             (elim_1 pre x)
-//             (elim_1 post x)
-//             (VSig.elim_vale_sig_cons hd tl args pre post v x)
+let rec lowstar_lemma
+          (dom:list td)
+          (code:V.va_code)
+          (args:list arg{List.length args + List.length dom < IX64.max_arity})
+          (num_stack_slots:nat)
+          (pre:VSig.vale_pre_tl dom)
+          (post:VSig.vale_post_tl dom)
+          (v:VSig.vale_sig_tl args (coerce code) pre post)
+    : lowstar_lemma_typ code args num_stack_slots pre post
+    = match dom with
+      | [] ->
+        lowstar_lemma_base code args num_stack_slots pre post v
+      | hd::tl ->
+        fun (x:td_as_type hd) ->
+          lowstar_lemma
+            tl
+            code
+            ((| hd, x |) :: args)
+            num_stack_slots
+            (elim_1 pre x)
+            (elim_1 post x)
+            (VSig.elim_vale_sig_cons hd tl args pre post v x)
 
 // let rec wrap_aux
 //          (code:V.va_code)
@@ -276,3 +374,50 @@ let lowstar_lemma_base
 //     (v:VSig.vale_sig pre post)
 //   : LSig.as_lowstar_sig code dom num_stack_slots pre post
 //   = wrap_aux code dom [] num_stack_slots (pre code) (post code) (v code IA.win)
+
+
+let test (l:B.loc) = assert (B.loc_disjoint l B.loc_none)
+let frame_mem_correspondence_pop
+       (args:list arg)
+       (h:HS.mem)
+       (va_s:V.va_state)
+ : Lemma
+     (requires
+       LSig.mem_correspondence args h va_s /\
+       B.loc_disjoint (LSig.mk_modifies_loc args)
+                      (B.loc_regions false (Set.singleton (HS.get_tip h))) /\
+       HS.poppable h)
+     (ensures
+       LSig.mem_correspondence args (HS.pop h) va_s)
+ = admit()
+
+module ST = FStar.HyperStack.ST
+let test (x:B.buffer bool)
+         (h:HS.mem{ B.live h x /\
+                    B.loc_disjoint (B.loc_buffer x)
+                                   (B.loc_regions false (Set.singleton (HS.get_tip h))) /\
+                    HS.poppable h }) =
+    B.popped_modifies h (HS.pop h);
+//    assume (B.modifies (B.loc_regions false (Set.singleton (HS.get_tip h))) h (HS.pop h)); //need this
+    assert (B.live (HS.pop h) x)
+
+
+        ST.equal_domains h1 h2 /\ HS.poppable h2})
+   : Lemma (B.loc_disjoint (B.loc_regions false (Set.singleton (HS.get_tip h1)))
+                           (B.loc_buffer x) /\
+            B.loc_disjoint (B.loc_regions false (Set.singleton (HS.get_tip h2)))
+                           (B.loc_buffer x) /\
+            B.live h2 x)
+
+let test (x:B.buffer bool)
+         (h0:HS.mem{B.live h0 x})
+         (h1:HS.mem{HS.fresh_frame h0 h1})
+         (h2:HS.mem{ST.equal_domains h1 h2 /\ HS.poppable h2})
+   : Lemma (B.loc_disjoint (B.loc_regions false (Set.singleton (HS.get_tip h1)))
+                           (B.loc_buffer x) /\
+            B.loc_disjoint (B.loc_regions false (Set.singleton (HS.get_tip h2)))
+                           (B.loc_buffer x) /\
+            B.live h2 x)
+            // B.live (HS.pop h2) x)
+   = ()
+//                          B.loc_none)= ()
